Fairness/MatchFinality.v
@@ -11,32 +11,45 @@ Definition final : LTL_formula := Atom p_terminal.
 
 Definition finalityOK : LTL_formula := G (Atom p_match_keep).
 
-Lemma matches_monotone : forall s m,
-  In m (matches s) -> In m (matches (step s)).
+Lemma matches_prefix : forall s,
+  prefix (matches s) (matches (step s)).
 Proof.
-  intros s m Hin.
+  intros s.
   unfold step.
-  destruct (phase s) eqn:Hp; simpl; try exact Hin.
+  destruct (phase s) eqn:Hp; simpl.
+  - exists []; reflexivity.
+  - exists []; reflexivity.
   - (* P3 -> either match_step or finish_matching *)
     destruct (match_step s) eqn:Hms; simpl.
-    + (* Some s' : use match_step_monotonic from Matching.v *)
-      apply (match_step_monotonic s s0 Hms).
-      exact Hin.
+    + (* Some s' : match_step appends one match *)
+      apply match_step_head_is_create in Hms.
+      destruct Hms as [b [a Hmatches]].
+      rewrite Hmatches. exists [create_match b a (matches s)]. reflexivity.
     + (* None : finish_matching; matches unchanged *)
-      exact Hin.
+      exists []; reflexivity.
+  - (* P4 *) exists []; reflexivity.
+  - (* P5 *) exists []; reflexivity.
+  - (* P6 *) exists []; reflexivity.
+  - (* P7 *) exists []; reflexivity.
 Qed.
 
 (* n-step: by simple induction using the one-step lemma. *)
-Theorem match_finality_after_n : forall n s m,
-  In m (matches s) -> In m (matches (execute n s)).
+Theorem match_finality_after_n : forall n s,
+  prefix (matches s) (matches (execute n s)).
 Proof.
-  induction n as [|n IH]; intros s m Hin; simpl; [exact Hin|].
-  apply IH. eapply matches_monotone; eauto.
+  induction n as [|n IH]; intros s; simpl.
+  - exists []; reflexivity.
+  - destruct (matches_prefix s) as [w' Hw'].
+    rewrite Hw'.
+    specialize (IH (step s)).
+    destruct IH as [w'' Hw''].
+    rewrite Hw''.
+    exists (w' ++ w''). rewrite app_assoc. reflexivity.
 Qed.
 
-Lemma matches_monotone_1 : forall s, matches_monotone_1_prop s.
+Lemma match_keep_prop_holds : forall s, match_keep_prop s.
 Proof.
-  intros s m Hin. now apply matches_monotone.
+  intro s. apply matches_prefix.
 Qed.
 
 Theorem match_finality_LTL : forall s,
@@ -46,5 +59,5 @@ Proof.
   rewrite satisfies_always_unfold.
   intros j _.
   apply (proj2 (mu_trace_atom_at_execute s j p_match_keep)).
-  unfold interp_atom. apply matches_monotone_1.
+  unfold interp_atom. apply match_keep_prop_holds.
 Qed.
